backend/Mach.v
@@ -313,10 +313,6 @@ Definition return_value (rs: regset) (sg: signature) :=
   | Twolong l1 l2 => Val.longofwords (rs l1) (rs l2)
   end.
 
-      (* forall (NO_CROSS_PTR: *)
-      (*     Genv.type_of_call ge (Genv.find_comp ge (Vptr f Ptrofs.zero)) cp = Genv.CrossCompartmentCall -> *)
-      (*     forall l, List.In l (regs_of_rpair (loc_result sg)) -> *)
-      (*         not_ptr (rs l)), *)
 (** Mach execution states. *)
 
 Inductive stackframe: Type :=
@@ -376,7 +372,10 @@ Definition parent_ra (s: list stackframe) : val :=
 
 Definition call_comp (s: list stackframe): compartment :=
   match parent_ra s with
-  | Vptr b _ => Genv.find_comp ge (Vptr b Ptrofs.zero)
+  | Vptr b _ => match Genv.find_comp ge (Vptr b Ptrofs.zero) with
+                | Some cp => cp
+                | None => default_compartment
+                end
   | _ => default_compartment
   end.
 
@@ -394,20 +393,20 @@ Inductive step: state -> trace -> state -> Prop :=
         E0 (State s f sp c rs m)
   | exec_Mgetstack:
       forall s f sp ofs ty dst c rs m v cp,
-      forall (CURCOMP: Genv.find_comp ge (Vptr f Ptrofs.zero) = cp),
+      forall (CURCOMP: Genv.find_comp ge (Vptr f Ptrofs.zero) = Some cp),
       load_stack m sp ty ofs (Some cp) = Some v ->
       step (State s f sp (Mgetstack ofs ty dst :: c) rs m)
         E0 (State s f sp c (rs#dst <- v) m)
   | exec_Msetstack:
       forall s f sp src ofs ty c rs m m' rs' cp,
-      forall (CURCOMP: Genv.find_comp ge (Vptr f Ptrofs.zero) = cp),
+      forall (CURCOMP: Genv.find_comp ge (Vptr f Ptrofs.zero) = Some cp),
       store_stack m sp ty ofs (rs src) cp = Some m' ->
       rs' = undef_regs (destroyed_by_setstack ty) rs ->
       step (State s f sp (Msetstack src ofs ty :: c) rs m)
         E0 (State s f sp c rs' m')
   | exec_Mgetparam:
       forall s fb f sp ofs ty dst c rs m (* cp' *) v rs' cp,
-      forall (CURCOMP: Genv.find_comp ge (Vptr fb Ptrofs.zero) = cp),
+      forall (CURCOMP: Genv.find_comp ge (Vptr fb Ptrofs.zero) = Some cp),
       Genv.find_funct_ptr ge fb = Some (Internal f) ->
       load_stack m sp Tptr f.(fn_link_ofs) (Some cp) = Some (parent_sp s) ->
       (* forall (COMPSP: call_comp s = Some cp'), *)
@@ -423,7 +422,7 @@ Inductive step: state -> trace -> state -> Prop :=
         E0 (State s f sp c rs' m)
   | exec_Mload:
       forall s f sp chunk addr args dst c rs m a v rs' cp,
-      forall (CURCOMP: Genv.find_comp ge (Vptr f Ptrofs.zero) = cp),
+      forall (CURCOMP: Genv.find_comp ge (Vptr f Ptrofs.zero) = Some cp),
       eval_addressing ge sp addr rs##args = Some a ->
       Mem.loadv chunk m a (Some cp) = Some v ->
       rs' = ((undef_regs (destroyed_by_load chunk addr) rs)#dst <- v) ->
@@ -431,7 +430,7 @@ Inductive step: state -> trace -> state -> Prop :=
         E0 (State s f sp c rs' m)
   | exec_Mstore:
       forall s f sp chunk addr args src c rs m m' a rs' cp,
-      forall (CURCOMP: Genv.find_comp ge (Vptr f Ptrofs.zero) = cp),
+      forall (CURCOMP: Genv.find_comp ge (Vptr f Ptrofs.zero) = Some cp),
       eval_addressing ge sp addr rs##args = Some a ->
       Mem.storev chunk m a (rs src) cp = Some m' ->
       rs' = undef_regs (destroyed_by_store chunk addr) rs ->
@@ -444,20 +443,21 @@ Inductive step: state -> trace -> state -> Prop :=
       return_address_offset f c ra ->
       forall (CALLED: Genv.find_funct_ptr ge f' = Some fd),
       forall (ALLOWED: Genv.allowed_call ge (comp_of f) (Vptr f' Ptrofs.zero)),
+      forall cp (CURCOMP: Genv.find_comp ge (Vptr f' Ptrofs.zero) = Some cp),
       (* call_arguments are never invalidated *)
       forall (ARGS: call_arguments (undef_regs destroyed_at_function_entry rs) m sp sig args),
       forall (NO_CROSS_PTR:
-          Genv.type_of_call ge (comp_of f) (Genv.find_comp ge (Vptr f' Ptrofs.zero)) = Genv.CrossCompartmentCall ->
+          Genv.type_of_call (comp_of f) cp = Genv.CrossCompartmentCall ->
           List.Forall not_ptr args),
-      forall (EV: call_trace ge (comp_of f) (Genv.find_comp ge (Vptr f' Ptrofs.zero)) (Vptr f' Ptrofs.zero)
+      forall (EV: call_trace ge (comp_of f) cp (Vptr f' Ptrofs.zero)
                args (sig_args sig) t),
       step (State s fb sp (Mcall sig ros :: c) rs m)
-        t (Callstate (Stackframe fb (Genv.find_comp ge (Vptr f' Ptrofs.zero)) sig sp ra c :: s)
+        t (Callstate (Stackframe fb cp sig sp ra c :: s)
                        f' sig rs m)
   | exec_Mtailcall:
       forall s fb stk soff sig ros c rs m f f' m' cp cp',
-      forall (CURCOMP: Genv.find_comp ge (Vptr fb Ptrofs.zero) = cp),
-      forall (NEXTCOMP: Genv.find_comp ge (Vptr f' Ptrofs.zero) = cp'),
+      forall (CURCOMP: Genv.find_comp ge (Vptr fb Ptrofs.zero) = Some cp),
+      forall (NEXTCOMP: Genv.find_comp ge (Vptr f' Ptrofs.zero) = Some cp'),
       find_function_ptr ge ros rs = Some f' ->
       Genv.find_funct_ptr ge fb = Some (Internal f) ->
       load_stack m (Vptr stk soff) Tptr f.(fn_link_ofs) (Some cp) = Some (parent_sp s) ->
@@ -469,7 +469,7 @@ Inductive step: state -> trace -> state -> Prop :=
         E0 (Callstate s f' sig rs m')
   | exec_Mbuiltin:
       forall s fb sp rs m ef args res b vargs t vres rs' m' cp,
-      forall (CURCOMP: Genv.find_comp ge (Vptr fb Ptrofs.zero) = cp),
+      forall (CURCOMP: Genv.find_comp ge (Vptr fb Ptrofs.zero) = Some cp),
       eval_builtin_args ge rs sp m args vargs ->
       external_call ef ge vargs m t vres m' ->
       forall ALLOWED: comp_of ef = cp,
@@ -508,7 +508,7 @@ Inductive step: state -> trace -> state -> Prop :=
   | exec_Mreturn:
       (* RB: NOTE: Think about compartment variables, here and in a similar case. *)
       forall s fb stk soff c rs m f m' retrs cp,
-      forall (CURCOMP: Genv.find_comp ge (Vptr fb Ptrofs.zero) = cp),
+      forall (CURCOMP: Genv.find_comp ge (Vptr fb Ptrofs.zero) = Some cp),
       Genv.find_funct_ptr ge fb = Some (Internal f) ->
       load_stack m (Vptr stk soff) Tptr f.(fn_link_ofs) (Some cp) = Some (parent_sp s) ->
       load_stack m (Vptr stk soff) Tptr f.(fn_retaddr_ofs) (Some cp) = Some (parent_ra s) ->
@@ -520,7 +520,7 @@ Inductive step: state -> trace -> state -> Prop :=
         E0 (Returnstate s retrs m')
   | exec_function_internal:
       forall s fb rs m f m1 m2 m3 stk callrs rs' cp sig,
-      forall (CURCOMP: Genv.find_comp ge (Vptr fb Ptrofs.zero) = cp),
+      forall (CURCOMP: Genv.find_comp ge (Vptr fb Ptrofs.zero) = Some cp),
       Genv.find_funct_ptr ge fb = Some (Internal f) ->
       Mem.alloc m cp 0 f.(fn_stacksize) = (m1, stk) ->
       let sp := Vptr stk Ptrofs.zero in
@@ -543,10 +543,11 @@ Inductive step: state -> trace -> state -> Prop :=
          t (Returnstate s rs' m')
   | exec_return:
       forall s f sp ra c rs m sg cp t,
+      forall cp' (CURCOMP: Genv.find_comp ge (Vptr f Ptrofs.zero) = Some cp'),
       forall (NO_CROSS_PTR:
-          Genv.type_of_call ge (Genv.find_comp ge (Vptr f Ptrofs.zero)) cp = Genv.CrossCompartmentCall ->
+          Genv.type_of_call cp' cp = Genv.CrossCompartmentCall ->
           not_ptr (return_value rs sg)),
-      forall (EV: return_trace ge (Genv.find_comp ge (Vptr f Ptrofs.zero)) cp (return_value rs sg) (sig_res sg) t),
+      forall (EV: return_trace ge cp' cp (return_value rs sg) (sig_res sg) t),
       step (Returnstate (Stackframe f cp sg sp ra c :: s) rs m)
         t (State s f sp c rs m).
 
